<?xml version="1.0" encoding="UTF-8"?>
<rdf:RDF xmlns:rdf="http://www.w3.org/1999/02/22-rdf-syntax-ns#"
  xmlns:owl="http://www.w3.org/2002/07/owl#"
  xmlns:dcterms="http://purl.org/dc/terms/"
  xmlns:vann="http://purl.org/vocab/vann/"
  xmlns:foaf="http://xmlns.com/foaf/0.1/"
  xmlns:dc="http://purl.org/dc/elements/1.1/"
  xmlns:adms="http://www.w3.org/ns/adms#"
  xmlns:rdfs="http://www.w3.org/2000/01/rdf-schema#">

  <owl:Ontology rdf:about="http://vocab.deri.ie/cpo">
    <rdf:type rdf:resource="http://www.w3.org/ns/adms#SemanticAsset"/>
    <dcterms:title>Client Permissions Ontology (CPO)</dcterms:title>
    <dcterms:description>The Client Permissions Ontology (CPO) is a light weight vocabulary that describes the scope and permissions which the resource owner grants to the client.</dcterms:description>
    <dcterms:modified rdf:datatype="http://www.w3.org/2001/XMLSchema#date">2013-05-02</dcterms:modified>
    <vann:preferredNamespaceUri>http://vocab.deri.ie/cpo#</vann:preferredNamespaceUri>
    <vann:preferredNamespacePrefix>cpo</vann:preferredNamespacePrefix>
    <foaf:homepage rdf:resource="http://vocab.deri.ie/cpo.html"/>
    <dcterms:created rdf:datatype="http://www.w3.org/2001/XMLSchema#date">2013-05-02</dcterms:created>
    <dcterms:publisher>http://vocab.deri.ie/cpo#DERI%2C%20NUI%20Galway</dcterms:publisher>
    <dcterms:partOf rdf:resource="http://vocab.deri.ie"/>
    <dcterms:type rdf:resource="http://purl.org/adms/assettype/Ontology"/>
    <dcterms:status rdf:resource="http://purl.org/adms/status/UnderDevelopment"/>
    <dc:creator rdf:resource="http://vocab.deri.ie/cpo#owesac"/>
  </owl:Ontology>

  <adms:SemanticDistribution rdf:about="http://vocab.deri.ie/cpo#ttl">
    <dcterms:FileFormat></dcterms:FileFormat>
    <adms:accessURL>http://vocab.deri.ie/cpo.ttl</adms:accessURL>
    <adms:status rdf:resource="http://purl.org/adms/status/Completed"/>
  </adms:SemanticDistribution>

  <adms:SemanticDistribution rdf:about="http://vocab.deri.ie/cpo#rdf">
    <dcterms:FileFormat></dcterms:FileFormat>
    <adms:accessURL>http://vocab.deri.ie/cpo.rdf</adms:accessURL>
    <adms:status rdf:resource="http://purl.org/adms/status/Completed"/>
  </adms:SemanticDistribution>

  <foaf:Person rdf:about="http://vocab.deri.ie/cpo#owesac">
    <foaf:name>Owen Sacco</foaf:name>
    <foaf:homepage rdf:resource="http://www.deri.ie/about/team/member/owen_sacco/"/>
  </foaf:Person>

  <dcterms:Agent rdf:about="http://vocab.deri.ie/cpo#DERI%2C%20NUI%20Galway">
    <foaf:member rdf:resource="http://vocab.deri.ie/cpo#owesac"/>
    <foaf:name>DERI, NUI Galway</foaf:name>
    <foaf:homepage rdf:resource="http://www.deri.ie/"/>
  </dcterms:Agent>

  <rdfs:Class rdf:about="http://vocab.deri.ie/cpo#ClientPermission">
    <rdf:type rdf:resource="http://www.w3.org/2002/07/owl#Class"/>
    <rdfs:label>Client Permission</rdfs:label>
    <rdfs:comment>The main class of CPO.</rdfs:comment>
  </rdfs:Class>

  <rdf:Property rdf:about="http://vocab.deri.ie/cpo#appliesToClient">
    <rdfs:label>applies to client</rdfs:label>
    <rdfs:comment>This property defines which client the scope and permissions apply to.</rdfs:comment>
    <rdfs:domain rdf:resource="http://vocab.deri.ie/cpo#ClientPermission"/>
  </rdf:Property>

  <rdf:Property rdf:about="http://vocab.deri.ie/cpo#hasPermission">
    <rdfs:label>has permission</rdfs:label>
    <rdfs:comment>This property defines the scope and permissions defined using the Privacy Preference Ontology (PPO).</rdfs:comment>
    <rdfs:domain rdf:resource="http://vocab.deri.ie/cpo#ClientPermission"/>
  </rdf:Property>

  <rdf:Property rdf:about="http://vocab.deri.ie/cpo#hasCredentials">
    <rdfs:label>has credentials</rdfs:label>
    <rdfs:comment>This property defines the request (temporary) token credentials and the access token credentials defined using the Credentials Ontology (CO).</rdfs:comment>
    <rdfs:domain rdf:resource="http://vocab.deri.ie/cpo#ClientPermission"/>
  </rdf:Property>

  <rdf:Property rdf:about="http://vocab.deri.ie/cpo#expireDateTime">
    <rdf:type rdf:resource="http://www.w3.org/2002/07/owl#DatatypeProperty"/>
    <rdfs:label>expire date time</rdfs:label>
    <rdfs:comment>This property defines when the scope and permissions expire.</rdfs:comment>
    <rdfs:domain rdf:resource="http://vocab.deri.ie/cpo#ClientPermission"/>
    <rdfs:range rdf:resource="http://www.w3.org/2000/01/rdf-schema#Literal"/>
  </rdf:Property>

</rdf:RDF>