<?xml version="1.0" encoding="UTF-8"?>
<rdf:RDF xmlns:rdf="http://www.w3.org/1999/02/22-rdf-syntax-ns#"
  xmlns:owl="http://www.w3.org/2002/07/owl#"
  xmlns:dcterms="http://purl.org/dc/terms/"
  xmlns:vann="http://purl.org/vocab/vann/"
  xmlns:foaf="http://xmlns.com/foaf/0.1/"
  xmlns:dc="http://purl.org/dc/elements/1.1/"
  xmlns:adms="http://www.w3.org/ns/adms#"
  xmlns:rdfs="http://www.w3.org/2000/01/rdf-schema#">

  <owl:Ontology rdf:about="http://vocab.deri.ie/pen">
    <rdf:type rdf:resource="http://www.w3.org/ns/adms#SemanticAsset"/>
    <dcterms:title>Process Energy Vocabulary</dcterms:title>
    <dcterms:description>pen : Process Energy, is a vocabulary used for describing the energy consumption of business processes.</dcterms:description>
    <dcterms:modified rdf:datatype="http://www.w3.org/2001/XMLSchema#date">2014-09-12</dcterms:modified>
    <vann:preferredNamespaceUri>http://vocab.deri.ie/pen#</vann:preferredNamespaceUri>
    <vann:preferredNamespacePrefix>pen</vann:preferredNamespacePrefix>
    <foaf:homepage rdf:resource="http://vocab.deri.ie/pen.html"/>
    <dcterms:created rdf:datatype="http://www.w3.org/2001/XMLSchema#date">2014-09-12</dcterms:created>
    <dcterms:partOf rdf:resource="http://vocab.deri.ie"/>
    <dcterms:type rdf:resource="http://purl.org/adms/assettype/Ontology"/>
    <dcterms:status rdf:resource="http://purl.org/adms/status/UnderDevelopment"/>
    <dc:creator rdf:resource="http://vocab.deri.ie/pen#wasder"/>
  </owl:Ontology>

  <adms:SemanticDistribution rdf:about="http://vocab.deri.ie/pen#ttl">
    <dcterms:FileFormat></dcterms:FileFormat>
    <adms:accessURL>http://vocab.deri.ie/pen.ttl</adms:accessURL>
    <adms:status rdf:resource="http://purl.org/adms/status/Completed"/>
  </adms:SemanticDistribution>

  <adms:SemanticDistribution rdf:about="http://vocab.deri.ie/pen#rdf">
    <dcterms:FileFormat></dcterms:FileFormat>
    <adms:accessURL>http://vocab.deri.ie/pen.rdf</adms:accessURL>
    <adms:status rdf:resource="http://purl.org/adms/status/Completed"/>
  </adms:SemanticDistribution>

  <foaf:Person rdf:about="http://vocab.deri.ie/pen#wasder">
    <foaf:name>Wassim Derguech</foaf:name>
    <foaf:homepage></foaf:homepage>
  </foaf:Person>

  <rdfs:Class rdf:about="http://vocab.deri.ie/pen#ConsumptionAmount">
    <rdf:type rdf:resource="http://www.w3.org/2002/07/owl#Class"/>
    <rdfs:label>Consumption Amount</rdfs:label>
    <rdfs:comment>This class describes the amount of energy consumed that has a value and unit of measurement.</rdfs:comment>
  </rdfs:Class>

  <rdfs:Class rdf:about="http://vocab.deri.ie/pen#EnergySource">
    <rdf:type rdf:resource="http://www.w3.org/2002/07/owl#Class"/>
    <rdfs:label>Energy Source</rdfs:label>
    <rdfs:comment>This class defines the source of energy being considered. This can be power, paper, etc.</rdfs:comment>
  </rdfs:Class>

  <rdfs:Class rdf:about="http://vocab.deri.ie/pen#EnergyConsumption">
    <rdf:type rdf:resource="http://www.w3.org/2002/07/owl#Class"/>
    <rdfs:label>Energy Consumption</rdfs:label>
    <rdfs:comment>This class represents the energy consumed.</rdfs:comment>
  </rdfs:Class>

  <rdf:Property rdf:about="http://vocab.deri.ie/pen#hasUnitOfMeasurement">
    <rdfs:label>hasUnitOfMeasurement</rdfs:label>
    <rdfs:comment>This property allows to determine the unit of measurement used.</rdfs:comment>
    <rdfs:domain rdf:resource="http://vocab.deri.ie/pen#ConsumptionAmount"/>
  </rdf:Property>

  <rdf:Property rdf:about="http://vocab.deri.ie/pen#hasValue">
    <rdf:type rdf:resource="http://www.w3.org/2002/07/owl#DatatypeProperty"/>
    <rdfs:label>hasValue</rdfs:label>
    <rdfs:domain rdf:resource="http://vocab.deri.ie/pen#ConsumptionAmount"/>
    <rdfs:range rdf:resource="http://www.w3.org/2001/XMLSchema#double"/>
    <rdfs:subPropertyOf rdf:resource="http://www.w3.org/2002/07/owl#hasValue"/>
  </rdf:Property>

  <rdf:Property rdf:about="http://vocab.deri.ie/pen#hasConsumptionAmount">
    <rdfs:label>hasConsumptionAmount</rdfs:label>
    <rdfs:comment>This property defines the amount of energy consumed.</rdfs:comment>
    <rdfs:domain rdf:resource="http://vocab.deri.ie/pen#EnergyConsumption"/>
    <rdfs:range rdf:resource="http://vocab.deri.ie/pen#ConsumptionAmount"/>
  </rdf:Property>

  <rdf:Property rdf:about="http://vocab.deri.ie/pen#hasEnergySource">
    <rdfs:label>hasEnergySource</rdfs:label>
    <rdfs:comment>This property allows to define what is the energy source is related to a particular consumption.</rdfs:comment>
    <rdfs:domain rdf:resource="http://vocab.deri.ie/pen#EnergyConsumption"/>
    <rdfs:range rdf:resource="http://vocab.deri.ie/pen#EnergySource"/>
  </rdf:Property>

  <rdf:Property rdf:about="http://vocab.deri.ie/pen#consumes">
    <rdfs:label>consumes</rdfs:label>
    <rdfs:comment>this property links the energy consumption to a particular business process task.</rdfs:comment>
    <rdfs:range rdf:resource="http://vocab.deri.ie/pen#EnergyConsumption"/>
  </rdf:Property>

</rdf:RDF>