<?xml version="1.0" encoding="UTF-8"?>
<rdf:RDF xmlns:rdf="http://www.w3.org/1999/02/22-rdf-syntax-ns#"
  xmlns:owl="http://www.w3.org/2002/07/owl#"
  xmlns:dcterms="http://purl.org/dc/terms/"
  xmlns:vann="http://purl.org/vocab/vann/"
  xmlns:foaf="http://xmlns.com/foaf/0.1/"
  xmlns:dc="http://purl.org/dc/elements/1.1/"
  xmlns:adms="http://www.w3.org/ns/adms#"
  xmlns:rdfs="http://www.w3.org/2000/01/rdf-schema#">

  <owl:Ontology rdf:about="http://vocab.deri.ie/slua">
    <rdf:type rdf:resource="http://www.w3.org/ns/adms#SemanticAsset"/>
    <dcterms:title>Semantically Linked Users and Actions</dcterms:title>
    <dcterms:description>SLUA (Semantically Linked Users and Actions) ontology aims to model users and tasks in crowdsourcing systems in terms of the human factors such as actions, capabilities, and rewards</dcterms:description>
    <dcterms:modified rdf:datatype="http://www.w3.org/2001/XMLSchema#date">2013-10-24</dcterms:modified>
    <vann:preferredNamespaceUri>http://vocab.deri.ie/slua#</vann:preferredNamespaceUri>
    <vann:preferredNamespacePrefix>slua</vann:preferredNamespacePrefix>
    <foaf:homepage rdf:resource="http://vocab.deri.ie/slua.html"/>
    <dcterms:created rdf:datatype="http://www.w3.org/2001/XMLSchema#date">2013-10-24</dcterms:created>
    <dcterms:publisher>http://vocab.deri.ie/slua#DERI%2C%20NUI%20Galway</dcterms:publisher>
    <dcterms:partOf rdf:resource="http://vocab.deri.ie"/>
    <dcterms:type rdf:resource="http://purl.org/adms/assettype/Ontology"/>
    <dcterms:status rdf:resource="http://purl.org/adms/status/UnderDevelopment"/>
    <dc:creator rdf:resource="http://vocab.deri.ie/slua#umahas"/>
  </owl:Ontology>

  <adms:SemanticDistribution rdf:about="http://vocab.deri.ie/slua#ttl">
    <dcterms:FileFormat></dcterms:FileFormat>
    <adms:accessURL>http://vocab.deri.ie/slua.ttl</adms:accessURL>
    <adms:status rdf:resource="http://purl.org/adms/status/Completed"/>
  </adms:SemanticDistribution>

  <adms:SemanticDistribution rdf:about="http://vocab.deri.ie/slua#rdf">
    <dcterms:FileFormat></dcterms:FileFormat>
    <adms:accessURL>http://vocab.deri.ie/slua.rdf</adms:accessURL>
    <adms:status rdf:resource="http://purl.org/adms/status/Completed"/>
  </adms:SemanticDistribution>

  <foaf:Person rdf:about="http://vocab.deri.ie/slua#umahas">
    <foaf:name>Umair ul Hassan</foaf:name>
    <foaf:homepage></foaf:homepage>
    <foaf:mbox rdf:resource="mailto:umair.ul.hassan@deri.org"/>
  </foaf:Person>

  <dcterms:Agent rdf:about="http://vocab.deri.ie/slua#DERI%2C%20NUI%20Galway">
    <foaf:member rdf:resource="http://vocab.deri.ie/slua#umahas"/>
    <foaf:name>DERI, NUI Galway</foaf:name>
    <foaf:homepage rdf:resource="http://www.deri.ie/"/>
  </dcterms:Agent>

  <rdfs:Class rdf:about="http://vocab.deri.ie/slua#Capability">
    <rdf:type rdf:resource="http://www.w3.org/2002/07/owl#Class"/>
    <rdfs:label>Capability</rdfs:label>
    <rdfs:comment>This class defines the human capability that is necessary for performing a task. Capability is defined as the ability of humans to do things in terms of both the capacity and the opportunity. </rdfs:comment>
  </rdfs:Class>

  <rdfs:Class rdf:about="http://vocab.deri.ie/slua#Reward">
    <rdf:type rdf:resource="http://www.w3.org/2002/07/owl#Class"/>
    <rdfs:label>Reward</rdfs:label>
    <rdfs:comment>This class represents the benefit associated with a task. It serves as an incentive for the participation in a crowdsourcing system. </rdfs:comment>
  </rdfs:Class>

  <rdfs:Class rdf:about="http://vocab.deri.ie/slua#Task">
    <rdf:type rdf:resource="http://www.w3.org/2002/07/owl#Class"/>
    <rdfs:label>Task</rdfs:label>
    <rdfs:comment>This class defines the unit of work, resulting in a desired outcome, that is assigned to the members of the crowd. A task may require one or more actions to produce a specific outcome. Therefore a task at the lowest level is composed of a set of actions. This class has composition relationship with itself because complex tasks can be broken down into small simple tasks.</rdfs:comment>
  </rdfs:Class>

  <rdfs:Class rdf:about="http://vocab.deri.ie/slua#Action">
    <rdf:type rdf:resource="http://www.w3.org/2002/07/owl#Class"/>
    <rdfs:label>Action</rdfs:label>
    <rdfs:comment>This class represents a specific act that is performed by the members (i.e. users) of the crowd. An action can be cognitive or physical. For instance, the comparison of two images involves a cognitive action from user.</rdfs:comment>
  </rdfs:Class>

  <rdfs:Class rdf:about="http://vocab.deri.ie/slua#User">
    <rdf:type rdf:resource="http://www.w3.org/2002/07/owl#Class"/>
    <rdfs:label>User</rdfs:label>
    <rdfs:comment>This class describes a human contributor in a crowdsourcing system. The user serves as an intelligent agent that is able to perform actions for successful completion of assigned tasks.</rdfs:comment>
  </rdfs:Class>

  <rdfs:Class rdf:about="http://vocab.deri.ie/slua#Ability">
    <rdf:type rdf:resource="http://www.w3.org/2002/07/owl#Class"/>
    <rdfs:label>Ability</rdfs:label>
    <rdfs:comment>This class represents the stable capacity of users to engage in a specific behaviour.</rdfs:comment>
    <rdfs:subClassOf rdf:resource="http://vocab.deri.ie/slua#Capability"/>
  </rdfs:Class>

  <rdfs:Class rdf:about="http://vocab.deri.ie/slua#Knowledge">
    <rdf:type rdf:resource="http://www.w3.org/2002/07/owl#Class"/>
    <rdfs:label>Knowledge</rdfs:label>
    <rdfs:comment>This class represents a body of information accumulated by users through education or experience.</rdfs:comment>
    <rdfs:subClassOf rdf:resource="http://vocab.deri.ie/slua#Capability"/>
  </rdfs:Class>

  <rdfs:Class rdf:about="http://vocab.deri.ie/slua#Skill">
    <rdf:type rdf:resource="http://www.w3.org/2002/07/owl#Class"/>
    <rdfs:label>Skill</rdfs:label>
    <rdfs:comment>This class represents the proficiency of a user in performing a task. Skill is acquired through training and practice.</rdfs:comment>
    <rdfs:subClassOf rdf:resource="http://vocab.deri.ie/slua#Capability"/>
  </rdfs:Class>

  <rdfs:Class rdf:about="http://vocab.deri.ie/slua#Location">
    <rdf:type rdf:resource="http://www.w3.org/2002/07/owl#Class"/>
    <rdfs:label>Location</rdfs:label>
    <rdfs:comment>This class represents a specific place where a user is or will be physically present. This type of capability enables crowd contributions that are related to a physical place such as participatory sensing.</rdfs:comment>
    <rdfs:subClassOf rdf:resource="http://vocab.deri.ie/slua#Capability"/>
  </rdfs:Class>

  <rdfs:Class rdf:about="http://vocab.deri.ie/slua#Availability">
    <rdf:type rdf:resource="http://www.w3.org/2002/07/owl#Class"/>
    <rdfs:label>Availability</rdfs:label>
    <rdfs:comment>This class represents the time interval or time instant during which a user is available to perform a task.</rdfs:comment>
    <rdfs:subClassOf rdf:resource="http://vocab.deri.ie/slua#Capability"/>
  </rdfs:Class>

  <rdfs:Class rdf:about="http://vocab.deri.ie/slua#Fun">
    <rdf:type rdf:resource="http://www.w3.org/2002/07/owl#Class"/>
    <rdfs:label>Fun</rdfs:label>
    <rdfs:comment>This class represents rewards involving entertainment value for users, such as games.</rdfs:comment>
    <rdfs:subClassOf rdf:resource="http://vocab.deri.ie/slua#Reward"/>
  </rdfs:Class>

  <rdfs:Class rdf:about="http://vocab.deri.ie/slua#Money">
    <rdf:type rdf:resource="http://www.w3.org/2002/07/owl#Class"/>
    <rdfs:label>Money</rdfs:label>
    <rdfs:comment>This class represents monetary rewards.</rdfs:comment>
    <rdfs:subClassOf rdf:resource="http://vocab.deri.ie/slua#Reward"/>
  </rdfs:Class>

  <rdfs:Class rdf:about="http://vocab.deri.ie/slua#Fame">
    <rdf:type rdf:resource="http://www.w3.org/2002/07/owl#Class"/>
    <rdfs:label>Fame</rdfs:label>
    <rdfs:comment>This class represents rewards that benefit people in terms of recognition.</rdfs:comment>
    <rdfs:subClassOf rdf:resource="http://vocab.deri.ie/slua#Reward"/>
  </rdfs:Class>

  <rdfs:Class rdf:about="http://vocab.deri.ie/slua#Altruism">
    <rdf:type rdf:resource="http://www.w3.org/2002/07/owl#Class"/>
    <rdfs:label>Altruism</rdfs:label>
    <rdfs:comment>This class represents rewards involving social good.</rdfs:comment>
    <rdfs:subClassOf rdf:resource="http://vocab.deri.ie/slua#Reward"/>
  </rdfs:Class>

  <rdfs:Class rdf:about="http://vocab.deri.ie/slua#Learning">
    <rdf:type rdf:resource="http://www.w3.org/2002/07/owl#Class"/>
    <rdfs:label>Learning</rdfs:label>
    <rdfs:comment>This class represents rewards resulting in personal improvement in skill or knowledge.</rdfs:comment>
    <rdfs:subClassOf rdf:resource="http://vocab.deri.ie/slua#Reward"/>
  </rdfs:Class>

  <rdf:Property rdf:about="http://vocab.deri.ie/slua#offers">
    <rdfs:label>offers</rdfs:label>
    <rdfs:comment>This property defines the relationship of Reward with Task. </rdfs:comment>
    <rdfs:domain rdf:resource="http://vocab.deri.ie/slua#Task"/>
    <rdfs:range rdf:resource="http://vocab.deri.ie/slua#Reward"/>
  </rdf:Property>

  <rdf:Property rdf:about="http://vocab.deri.ie/slua#possesses">
    <rdfs:label>possesses</rdfs:label>
    <rdfs:comment>This relation describes a User who has one or more capabilities.</rdfs:comment>
    <rdfs:domain rdf:resource="http://vocab.deri.ie/slua#User"/>
    <rdfs:range rdf:resource="http://vocab.deri.ie/slua#Capability"/>
  </rdf:Property>

  <rdf:Property rdf:about="http://vocab.deri.ie/slua#performs">
    <rdfs:label>performs</rdfs:label>
    <rdfs:comment>This relation exists between a User who performs for actions that are required for generating the desired outcome of a task.</rdfs:comment>
    <rdfs:domain rdf:resource="http://vocab.deri.ie/slua#User"/>
    <rdfs:range rdf:resource="http://vocab.deri.ie/slua#Action"/>
  </rdf:Property>

  <rdf:Property rdf:about="http://vocab.deri.ie/slua#earns">
    <rdfs:label>earns</rdfs:label>
    <rdfs:comment>The relation between a user who is interested in a particular reward is described with this property.</rdfs:comment>
    <rdfs:domain rdf:resource="http://vocab.deri.ie/slua#User"/>
    <rdfs:range rdf:resource="http://vocab.deri.ie/slua#Reward"/>
  </rdf:Property>

  <rdf:Property rdf:about="http://vocab.deri.ie/slua#isConnectedWith">
    <rdfs:label>isConnectedWith</rdfs:label>
    <rdfs:domain rdf:resource="http://vocab.deri.ie/slua#User"/>
    <rdfs:range rdf:resource="http://vocab.deri.ie/slua#User"/>
  </rdf:Property>

  <rdf:Property rdf:about="http://vocab.deri.ie/slua#includes">
    <rdfs:label>includes</rdfs:label>
    <rdfs:comment>A Task can include one or more actions that a User needs to perform for successful completion of the Task.</rdfs:comment>
    <rdfs:domain rdf:resource="http://vocab.deri.ie/slua#Task"/>
    <rdfs:range rdf:resource="http://vocab.deri.ie/slua#Action"/>
  </rdf:Property>

  <rdf:Property rdf:about="http://vocab.deri.ie/slua#requires">
    <rdfs:label>requires</rdfs:label>
    <rdfs:comment>A Task can define requirements of one or more human capabilities using this property.</rdfs:comment>
    <rdfs:domain rdf:resource="http://vocab.deri.ie/slua#Task"/>
    <rdfs:range rdf:resource="http://vocab.deri.ie/slua#Capability"/>
  </rdf:Property>

  <rdf:Property rdf:about="http://vocab.deri.ie/slua#isPartOf">
    <rdfs:label>isPartOf</rdfs:label>
    <rdfs:comment>A complex Task can be decomposed into small manageable tasks. Therefore this property helps is describing the composition relationship between tasks.</rdfs:comment>
    <rdfs:domain rdf:resource="http://vocab.deri.ie/slua#Task"/>
    <rdfs:range rdf:resource="http://vocab.deri.ie/slua#Task"/>
  </rdf:Property>

</rdf:RDF>