<?xml version="1.0" encoding="UTF-8"?>
<rdf:RDF xmlns:rdf="http://www.w3.org/1999/02/22-rdf-syntax-ns#"
  xmlns:owl="http://www.w3.org/2002/07/owl#"
  xmlns:dcterms="http://purl.org/dc/terms/"
  xmlns:vann="http://purl.org/vocab/vann/"
  xmlns:foaf="http://xmlns.com/foaf/0.1/"
  xmlns:dc="http://purl.org/dc/elements/1.1/"
  xmlns:adms="http://www.w3.org/ns/adms#"
  xmlns:rdfs="http://www.w3.org/2000/01/rdf-schema#">

  <owl:Ontology rdf:about="http://vocab.deri.ie/wsapo">
    <rdf:type rdf:resource="http://www.w3.org/ns/adms#SemanticAsset"/>
    <dcterms:title>Web Service Authorisation Preferences Ontology (WSAPO)</dcterms:title>
    <dcterms:description>The Web Service Authorisation Preferences Ontology (WSAPO) is a light weight vocabulary that describes the details of the Web Service Authorisation component which are stored on the client side. These details are used by the client during the authorisation process.</dcterms:description>
    <dcterms:modified rdf:datatype="http://www.w3.org/2001/XMLSchema#date">2013-05-02</dcterms:modified>
    <vann:preferredNamespaceUri>http://vocab.deri.ie/wsapo#</vann:preferredNamespaceUri>
    <vann:preferredNamespacePrefix>wsapo</vann:preferredNamespacePrefix>
    <foaf:homepage rdf:resource="http://vocab.deri.ie/wsapo.html"/>
    <dcterms:created rdf:datatype="http://www.w3.org/2001/XMLSchema#date">2013-05-02</dcterms:created>
    <dcterms:publisher>http://vocab.deri.ie/wsapo#DERI%2C%20NUI%20Galway</dcterms:publisher>
    <dcterms:partOf rdf:resource="http://vocab.deri.ie"/>
    <dcterms:type rdf:resource="http://purl.org/adms/assettype/Ontology"/>
    <dcterms:status rdf:resource="http://purl.org/adms/status/UnderDevelopment"/>
    <dc:creator rdf:resource="http://vocab.deri.ie/wsapo#owesac"/>
  </owl:Ontology>

  <adms:SemanticDistribution rdf:about="http://vocab.deri.ie/wsapo#ttl">
    <dcterms:FileFormat></dcterms:FileFormat>
    <adms:accessURL>http://vocab.deri.ie/wsapo.ttl</adms:accessURL>
    <adms:status rdf:resource="http://purl.org/adms/status/Completed"/>
  </adms:SemanticDistribution>

  <adms:SemanticDistribution rdf:about="http://vocab.deri.ie/wsapo#rdf">
    <dcterms:FileFormat></dcterms:FileFormat>
    <adms:accessURL>http://vocab.deri.ie/wsapo.rdf</adms:accessURL>
    <adms:status rdf:resource="http://purl.org/adms/status/Completed"/>
  </adms:SemanticDistribution>

  <foaf:Person rdf:about="http://vocab.deri.ie/wsapo#owesac">
    <foaf:name>Owen Sacco</foaf:name>
    <foaf:homepage rdf:resource="http://www.deri.ie/about/team/member/owen_sacco/"/>
  </foaf:Person>

  <dcterms:Agent rdf:about="http://vocab.deri.ie/wsapo#DERI%2C%20NUI%20Galway">
    <foaf:member rdf:resource="http://vocab.deri.ie/wsapo#owesac"/>
    <foaf:name>DERI, NUI Galway</foaf:name>
    <foaf:homepage rdf:resource="http://www.deri.ie/"/>
  </dcterms:Agent>

  <rdfs:Class rdf:about="http://vocab.deri.ie/wsapo#WebService">
    <rdf:type rdf:resource="http://www.w3.org/2002/07/owl#Class"/>
    <rdfs:label>Web Service</rdfs:label>
    <rdfs:comment>The main class of WSAPO.</rdfs:comment>
  </rdfs:Class>

  <rdf:Property rdf:about="http://vocab.deri.ie/wsapo#hasCredentials">
    <rdfs:label>has credentials</rdfs:label>
    <rdfs:comment>A property that defines the client's credentials (generated by a particular Web Service) which are used during the authorisation process. The credentials are described using the Credentials Ontology (CO).</rdfs:comment>
    <rdfs:domain rdf:resource="http://vocab.deri.ie/wsapo#WebService"/>
  </rdf:Property>

  <rdf:Property rdf:about="http://vocab.deri.ie/wsapo#hasTemporaryTokenEndpoint">
    <rdfs:label>has temporary token endpoint</rdfs:label>
    <rdfs:comment>This property defines the Web Service's endpoint for generating the request (temporary) token credentials.</rdfs:comment>
    <rdfs:domain rdf:resource="http://vocab.deri.ie/wsapo#WebService"/>
    <rdfs:range rdf:resource="http://www.w3.org/2000/01/rdf-schema#Resource"/>
  </rdf:Property>

  <rdf:Property rdf:about="http://vocab.deri.ie/wsapo#hasAccessTokenEndpoint">
    <rdfs:label>has access token endpoint</rdfs:label>
    <rdfs:comment>A property that defines the Web Service's endpoint to exchange the request (temporary) token credentials to access token credentials.</rdfs:comment>
    <rdfs:domain rdf:resource="http://vocab.deri.ie/wsapo#WebService"/>
    <rdfs:range rdf:resource="http://www.w3.org/2000/01/rdf-schema#Resource"/>
  </rdf:Property>

  <rdf:Property rdf:about="http://vocab.deri.ie/wsapo#hasAuthoriseEndpoint">
    <rdfs:label>has authorise endpoint</rdfs:label>
    <rdfs:comment>A property that defines the Web Service's authorisation endpoint.</rdfs:comment>
    <rdfs:domain rdf:resource="http://vocab.deri.ie/wsapo#WebService"/>
    <rdfs:range rdf:resource="http://www.w3.org/2000/01/rdf-schema#Resource"/>
  </rdf:Property>

</rdf:RDF>